\documentclass{article}
\usepackage{ifthen}
\usepackage{epsfig}
\usepackage[utf8]{inputenc}
\usepackage{newunicodechar}
  \newunicodechar{⁻}{${}^{-}$}% Superscript minus
  \newunicodechar{²}{${}^{2}$}% Superscript two
  \newunicodechar{³}{${}^{3}$}% Superscript three

\pagestyle{empty}
\begin{document}
$H_{2}^{+}$
\pagebreak

$H_{2}$
\pagebreak

$\hat{H}$
\pagebreak

$E_{gs}$
\pagebreak

$\Psi$
\pagebreak

\begin{equation}E_{gs} \leq \langle \Psi | \hat{H} | \Psi \rangle \equiv \langle \hat{H} \rangle, \end{equation}
\pagebreak

$ E_{gs}$
\pagebreak

$\langle \hat{H} \rangle$
\pagebreak

\begin{align*}\tag 1 \langle \hat{H} \rangle & = \langle \Psi |\hat{H}| \Psi \rangle \\ & = \int \Psi^* \hat{H} \Psi d\textbf{r}_i, \end{align*}
\pagebreak

$\textbf{r}_i$
\pagebreak

$ H_2^+ $
\pagebreak

$ H_2 $
\pagebreak

\begin{equation}\tag {2} \hat{H}(\{\textbf{r}_i\},\{\textbf{R}_I\})\Psi(\{\textbf{r}_i\}) \equiv\left(-\frac{1}{2}\sum_i\nabla_i^2+\sum_{i>j}\frac{1}{r_{ij}}-\sum_{I}\sum_{i}\frac{Z_I}{r_{iI}}\right)\Psi=E\Psi, \end{equation}
\pagebreak

$N_n$
\pagebreak

$Z_I $
\pagebreak

$\textbf{R}_I $
\pagebreak

$N $
\pagebreak

$\textbf{r}_i $
\pagebreak

$ r_{ij} = \left | \textbf{r}_i - \textbf{r}_j \right | $
\pagebreak

$r_{iI}= \left | \textbf{r}_i - \textbf{R}_I \right | $
\pagebreak

\begin{equation}\tag {3} \langle \hat{H}_L \rangle_{|\Psi|^2} = \frac{\int |\Psi|^2(\hat{H}\Psi)/\Psi d\{\textbf{r}_i\}}{\int |\Psi|^2 d{\textbf{r}_i}}, \end{equation}
\pagebreak

$ \hat{H}_L = \hat{H}\Psi / \Psi $
\pagebreak

$3N$
\pagebreak

$\{\phi_k\}_{k=1}^{M}$
\pagebreak

$ \textbf{0} $
\pagebreak

$ \{\phi_k^I(\textbf{r})=\phi_k(\textbf{r}-\textbf{R}_I)\}_{k=1}^{M} $
\pagebreak

\begin{equation}\{\varphi_k(\textbf{r})\}_{k=1}^{N_nM} = \bigcup_I\{\phi_k^I(\textbf{r})\}. \end{equation}
\pagebreak

\begin{equation} \psi_i(\textbf{r})=\sum_{k=1}^{N_IM}c_{ik}\varphi_k(\textbf{r}). \end{equation}
\pagebreak

$ \Psi=\psi_1 $
\pagebreak

$N_n\times M $
\pagebreak

\begin{equation} H\psi_1(\textbf{r})=\sum_kc_{ik}H\varphi_k(\textbf{r}),\end{equation}
\pagebreak

$H\varphi_k(\textbf{r})$
\pagebreak

$N > 1$
\pagebreak

\begin{equation} \Psi(\{\textbf{r}_i\})=e^{J(\{\textbf{r}_i\})}D(\{\psi_i\},\{\textbf{r}_i\}), \end{equation}
\pagebreak

\begin{equation} D(\{\psi_i\},\{\textbf{r}_i\})=\begin{vmatrix} \psi_1(\textbf{r}_1) &\psi_2(\textbf{r}_1) &\cdots& \psi_N(\textbf{r}_1) \\ \psi_1(\textbf{r}_2) &\psi_2(\textbf{r}_2) &\cdots& \psi_N(\textbf{r}_2) \\ \vdots &\vdots &\ddots&\vdots \\ \psi_1(\textbf{r}_N) &\psi_2(\textbf{r}_N) &\cdots& \psi_N(\textbf{r}_N) \\ \end{vmatrix}. \end{equation}
\pagebreak

$M\times N_n\times N+N_J$
\pagebreak

$ N_J $
\pagebreak

$J$
\pagebreak

$\{\psi_i\}$
\pagebreak

$\psi_1(\textbf{r},\uparrow)=\psi_1(\textbf{r})|{\uparrow}\rangle$
\pagebreak

$\psi_2=\psi_1|{\downarrow}\rangle $
\pagebreak

\begin{equation} D(\{\psi_i\},\{\textbf{r}_i\})=\psi_1(\textbf{r}_1)\psi_2(\textbf{r}_2)-\psi_1(\textbf{r}_2)\psi_2(\textbf{r}_1)=\psi_1(\textbf{r}_1)\psi_1(\textbf{r}_2)(|{\uparrow}\rangle|{\downarrow}\rangle-|{\downarrow}\rangle|{\uparrow}\rangle)=\psi_1(\textbf{r}_1)\psi_1(\textbf{r}_2).\end{equation}
\pagebreak

\begin{equation} J(\{\textbf{r}_i\})=\sum_I\sum_{i<j}U_{Iij}, \end{equation}
\pagebreak

\begin{equation} U_{Iij} = \sum_k \Delta(m_{kI},n_{kI})c_{kI}(\bar{r}_{iI}^{m_{kI}}\bar{r}_{jI}^{n_{kI}}+\bar{r}_{jI}^{m_{kI}}\bar{r}_{iI}^{n_{kI}})\bar{r}_{ij}^{o_{kI}}, \end{equation}
\pagebreak

\begin{equation} \bar{r}_{iI} =\frac{b_Ir_{iI}}{1+b_{I}r_{iI}}, \end{equation}
\pagebreak

\begin{equation} \bar{r}_{ij}=\frac{d_Ir_{ij}}{1+d_{I}r_{ij}}, \end{equation}
\pagebreak

\begin{equation} \Delta(m,n)=1-0.5\delta_{mn}, \end{equation}
\pagebreak

$(m,n,o)$
\pagebreak

$\{b_I,d_I,\{c_{kI}\}\}$
\pagebreak

$N_J=N_n(N_u+2)$
\pagebreak

\end{document}
